\input{h.tex}
\BeginDoc{}
\def\dec{\left| 
\begin{array}{ccc}}
\def\dee{\end{array}
\right|}
\def\d{\rm d}
\section{Mocniny, mocninná funkce}
\pd{10-1.pdf}
$$
\f{
	(a+b)^m(a-b)^m(x-y)^{mn}(x+y)^{nm}(a-b)^m
	}{
		(x-y)^{nm}(a+b)^m(x+y)^{nm}
	}
	=
	(a-b)^{2m}
	$$
\pd{10-2.pdf}
$$
a^{2x+3y-5x+y-4x-5y+8x+2y} b^{4x-5y-3x-y-2x+4y+x+2y}
=
a^{x+y}b^{0} = a^{x+y}
$$
\pd{10-3.pdf}
Nechť $k=a^x$ a $l=b^y$:
$$
\f{
	(l+\f 1 l)(k^2-2+\f2{k^2})(l^2-2l+1)(k^2+1)
}{
	(k+\f 1 k)(l^2-2+\f1{l^2})(k^2-2k+1)(l^2+1)
}
=
\f{
	(l^3-2l^2+2l-2+\f1 l)(k^4-k^2+\f1{k^2})
}{
	(k^3-kl^2+2k-2+\f1 k)(l^4-l^2+\f1{l^2})
}
=$$
$$=
\f{
	(b^{3y}-2b^{2y}+2b^y-2+\f1 {b^y})(a^{4x}-a^{2x}+\f1{a^{2x}})
}{
	(a^{3x}-2a^{2x}+2a^x-2+\f1 {a^x})(b^{4y}-b^{2y}+\f1{b^{2y}})
}
$$

\pd[0.5]{10-4.pdf}
$$
a^{\f n {n-1}} - xa^{\f{1}{n-1}} -ax^{\f 1 {n-1}} +xx^{\f1{n-1}} 
=
aa^{\f 1 {n-1}} - xa^{\f{1}{n-1}} -ax^{\f 1 {n-1}} +xx^{\f 1{n-1}} 
=
(a -\sqrt{n-1} x)
(\sqrt[n-1] a -x )
$$
\pd[0.3]{10-6.pdf}
\def\s{\sqrt}
$$
\f {12}{\s 2 + \s 3 -\s 5} \* \f{\s2+\s3+\s5}{\s2+\s3+\s5}
=
\f{12(\s2+\s3+\s5)}{(\s 2 +\s 3)^2+5}
=
\f{12(\s2+\s3+\s5)}{( 5 +\s{12})^2+5}
=
\f{12(\s2+\s3+\s5)}{5+\s{12}+5} \*\f{10-\s{12}}{10-\s{12}}
=
\f{12(\s2+\s3+\s5)(10-\s{12}}{100-12}
=
\f{3(\s2+\s3+\s5)(10-\s{12}}{22}
$$

\pd[0.2]{10-7.pdf}
$$
\f{\s 3 + 1}{(\s 2 -1)(\s 3 +1)} \*\f{\s2-1}{\s 2+1}
=
1
$$
\pd{10-8.pdf}
$$\f{(a-x)(a+x)}{2\s[3]a\s[3]x (\s[3]a-\s[3]x)(\s[3]a+\s[3]x)}
=
\f{a^2-x^2}{2a\s[3]x-2x\s[3]a}
$$
\pd{10-9.pdf}
$$
\(\f{5+2\s{15}+3+5-2\s{15}+3}{5-3}\)^3
+
\(\f{6-3\sqrt3}{4-3}+3\sqrt 3\)^4
=
\(\f{16}{2}\)^3
+
\(6\)^4
=8^3+6^4
$$
\pd{10-11.pdf}
\begin{enumerate}
	\item 
		Když $x>0$: $y=\f{2}{2x-2} = \f 1{x-1}$\\
		Rovnoosá hyperbola se středem $[1;0]$.

		Když $x\le0$: $y=\f2{-2}=-1$.
	\item
		Když $x\ge2$: $-\sqrt{2(x-x+2)} = -2$
		Když $x\le2$: $-\sqrt{2(x+x-2)} = -2\sqrt{x+1}$
		Odmocniná funkce s počátkem $[1;0]$.
\end{enumerate}

\pd{10-11r.pdf}
\EndDoc
