\input{h.tex}
\BeginDoc{}
\def\dec{\left| 
\begin{array}{ccc}}
\def\dee{\end{array}
\right|}
\def\d{\rm d}
\section{Logaritmus, logaritmická funkce}
\pd{12-1.pdf}
$$\f{\log_ax\*\log_bx}{\log_a x + \log_b x}  = \f{1}{\f{1}{\log_a x}+\f1{\log_b x}} = \f1{\log_x a+\log_x b}=\f1{\log_x ab} = \log_{ab} x$$
\pd{12-2.pdf}
$$\f{\log_a x}{1+\log_ab} = \f{\log_a x\*\log_x a}{\log_x a + \log_x a \log_a b}= \f1{\log_x a+\log_x b}=\f1{\log_x ab} = \log_{ab} x$$
\pd{12-3.pdf}
$0< n = \f{z+1}{z-1} \imp z \not \in \<-1;1\>$

$x^4-25x^2+72=72$:\\
$x^4-25x^2=0$\\
$x^2(x^2-25)=0$\\
$x^2(x-5)(x+5)=0$


$x^4-25x^2+72=-72$:\\
$D=25^2-8\*72 = 49 = 7^2$
$(x^2-9)(x^2-16)=0$\\
$(x+3)(x-3)(x+4)(x-4)=0$

Log je difinovaný když:
$x\in (-\infty;5)\cup(-4;-3)\cup(3;4)\cup(5;\infty)$

\pd{12-4.pdf}
$$x=z^{\f 14 \log_z a + \log_z \log _z  b}$$
$$x=z^{\f 14 \log_z a}z^{\log_z \log _z  b}$$
$$x=a z^{\f 14}z \log_z b$$
\pd{12-5.pdf}
$$\log_a(x^2+x) < \log_a{2x+6}$$
\begin{enumerate}
	\item [$a<1$]
		$$x^2+x>2x+6$$
		$$x^2-x-6>0$$
		$$(x-3)(x+2)>0$$

		$x\in(-\infty;-2)\cap(3;\infty)$
	\item [$a>1$]
		$$x^2+x<2x+6$$
		$$x^2-x-6<0$$
		$$(x-3)(x+2)<0$$

		$x\in(-2;3)$
\end{enumerate}

\pd{12-6.pdf}
$$3\log_4\pi<\f 52$$
$$\log_4\pi<\f 56$$
$$\pi<4^{\f 56}$$
$$\pi<4^{\f 56}= 2\*4^{\f 13}$$
$$\pi<2. < 3.16 = 2\*1.58 = 2\*3.9444312^{\f 13} < 2\* 4^{\f 13}$$
\newpage
\pd{12-7.pdf}
\pd{12-8.pdf}
\pd{12-r1.pdf}
\pd{12-9.pdf}
\pd{12-10.pdf}
\pd{12-r2.pdf}
\newpage\ \\[-50pt]
\pd{12-11.pdf}
\pd{12-12.pdf}
\pd{12-r3.pdf}
\EndDoc
