\input{h.tex}
\BeginDoc{}
\def\posloup{$\zs{a_n}_{n=1}^{\infty}$}
\def\pos#1{\zs{#1}_{n=1}^{\infty}}
\def\li{\lim_{n\rightarrow\infty}}
\def\lix{\lim_{x\rightarrow x_0}}
\def\r{\rightarrow}
\def\sup{{\rm sup\ }}
\def\sciwinfup{{\rm inf\ }}
\def\su{\sum_{n=1}^{\infty}}
\Pr
$$\lim_{x\r 0} x\sin\f1x = 0$$

\Pr
$$
\lim{x\r 2} \f{x-2}{x^2-3x+2}
=
\lim{x\r 2} \f{x-2}{(x-2)(x-1)}
=
\lim{x\r 2} \f{1}{(x-1)}
= 1
$$

$$
\lim_{x\r -3} \f{3x^2+11x+6}{x^3+27}
=
\lim_{x\r -3} \f{3x-2}{1x^2-3x+9} =\f{-11}{27}
$$

$$
\lim_{x\r \pi} \f{\tg x}{\sin 2x} 
=
\lim_{x\r \pi} \f{\sin x}{2\sin x \cos x \cos x} 
=
\lim_{x\r \pi} \f{1}{2\cos x \cos x} = \f 12
$$

$$
\lim_{x\r\f\pi4} \f{\sin x-\cos x}{\cos 2x}
=
\lim_{x\r\f\pi4} \f{\sin x-\cos x}{\cos^2 x-\sin^2 x}
=
\lim_{x\r\f\pi4} \f{-1}{\cos x+\sin x}
=
-1
$$

\Pr
$$
\lim_{x\r6} \f{x-6}{\sqrt{x+3}-3}
=
\lim_{x\r6} \f{x-6}{x+3-9} (\sqrt{x+3}+3)
=
\sqrt{9} + 3
=
6
$$

$$
\lim_{x\r 0} \f{\sqrt{x^2+1}-1}{\sqrt{x^2+16}-4}
=
\lim_{x\r 0} \f{\sqrt{x^2+1}-1}{x^2+16-16}(\sqrt{x^2+16}+4)
=
\lim_{x\r 0} \f{\sqrt{x^2+1}-1}{x^2}(\sqrt{x^2+16}+4)
=$$$$=
\lim_{x\r 0} \sqrt{\f{x^2+1}{x^4}}(\sqrt{x^2+16}+4)
=
\lim_{x\r 0} \sqrt{\f{x^2}{x^4}}(\sqrt{x^2+16}+4)
=
\lim_{x\r 0} \sqrt{\f{1}{x^2}}(\sqrt{x^2+16}+4)
=8
$$

$$
\lim_{x\r -1}\f{x^3+1}{\sqrt{x^2-3x}+2x}
=
\lim_{x\r -1}\f{x^3+1}{x^2-3x-4x^2}\*\sqrt{x^2-3x}-2x
=$$$$=
\lim_{x\r -1}\f{x^3+1}{-3x(1+x)}\*\sqrt{x^2-3x}-2x
=
\lim_{x\r -1}\f{x^2-x+1}{-3x}\*\sqrt{x^2-3x}-2x
=
\f{1}3(2+2)=\f 43
$$

$$
\lim_{x\r 1} \f{2-\sqrt{x+3}}{x^3-1}
=
\lim_{x\r 1} \f{4-x-3}{(x-1)(x^2+x+1)(2+\sqrt{x+3}}
=
\lim_{x\r 1} \f{-1}{(x^2+x+1)(2+\sqrt{x+3}}
=
\f{-1}{12}
$$
\Pr
$0;\f 3 5 ; +\infty;+\infty$
\Pr

\Pr
$$
\lim_{x\r-\infty} (\sqrt{x^2+4}+x)
=
\lim_{x\r\infty} (\sqrt{x^2+4}-x)
=
\lim_{x\r\infty} \f{x^2-x^2+4}{\sqrt{x^2+4}+x}
=0
$$

\Pr
$$\lim_{x\r+\infty} \f{\sin 5x}{x} =0$$

$$\lim_{x\r0} x\cos \f  1 x = 0$$


\EndDoc
